
LAB 9

SUBMISSION INSTRUCTIONS

Submit your lab files `lab9_exercise1.m` and `lab9_exercise2.m` by attaching them to an **email with the subject Lab9-ID** where ID stands for your roll number (for example, if your roll number is 123456, then the subject will be `Lab9_123456`) and send it to

`mth430.iitk@gmail.com`

before 11:59 pm on October 17, 2019.

LAB EXERCISES

Consider the problem

$$\begin{aligned}u_t(t, x) + u_x(t, x) &= 0, \quad x \in (-1, 1), \quad t > 0, \\u(0, x) &= \exp(-100x^2), \quad x \in [-1, 1], \\u(t, -1) &= \exp(-100(1+t)^2), \quad t > 0, \\u(t, 1) &= \exp(-100(1-t)^2), \quad t > 0.\end{aligned}$$

Clearly, $u_e(t, x) = e^{-100(x-t)^2}$ is the exact solution. Write a function `lab9_exercise1` in the following format

```
function [ ] = lab9_exercise1(nt,nx,cfl)
```

to implement its numerical solution using the forward-centered difference scheme

$$u_j^{n+1} = u_j^n - \frac{\Delta t}{2\Delta x} (u_{j+1}^n - u_{j-1}^n).$$

The input parameters `nt` and `nx`, respectively, specify the number of time steps N_t to reach the final time $T = N_t \Delta t$, and the number N_x used to define $\Delta x = 2/N_x$ so that the x -grid points $x_j = -1 + j\Delta x, j = 0, \dots, N_x$. The input `cfl` specifies the ratio $\Delta t/\Delta x$.

Next, solve the same problem using the upstream/upwind (forward-backward) method that reads

$$u_j^{n+1} = u_j^n - \frac{\Delta t}{\Delta x} (u_j^n - u_{j-1}^n).$$

Your implementation of this scheme should read

function [] = lab9_exercise2(nt,nx,cfl)

where the input parameters remain the same as those in `lab9_exercise1.m`. Both these implementations should display the evolution of the solution as a movie by plotting the solution at successive time steps on the same figure.

OTHER EXERCISES

1. To show that the finite difference scheme

$$u_j^{n+1} = u_j^n - \frac{\Delta t}{2\Delta x} (u_{j+1}^n - u_{j-1}^n)$$

is divergent, complete the following steps:

- (a) Show that $e^{\beta t} e^{i\alpha x}$ is a solution to the difference equation if

$$e^{\beta \Delta t} = 1 + i \frac{\Delta t}{\Delta x} \sin(\alpha \Delta x).$$

- (b) Consider the initial data

$$u_0(x) = \sum_{k=0}^{\infty} 2^{-2k} \cos(2^{k-1}\pi x)$$

Show that

$$u(t, x) = \operatorname{Re} \sum_{k=0}^{\infty} 2^{-2k} e^{\beta_k t} e^{i\alpha_k x}$$

solves the difference equation along with the initial data where, for $\alpha_k = 2^{k-1}\pi$, β_k is chosen such that it satisfies the identity in part (a).

- (c) Take $\Delta x = 2^{-n}$. Show that the term $k = n$ dominates the sum of all the other terms as $n \rightarrow \infty$, in

$$u(t, 0) \geq - \sum_{k=n+1}^{\infty} 2^{-2k} + \operatorname{Re} \sum_{k=0}^n 2^{-2k} \left(1 + i \frac{\Delta t}{\Delta x} \sin(2^{k-1-n}\pi) \right)^{t/\Delta t}.$$

Conclude that $u(t, 0) \rightarrow \infty$ as $n \rightarrow \infty$.

2. Investigate the consistency, order, and stability of the following schemes

- (a)

$$u_j^{n+1} = u_j^n - \frac{\Delta t}{2\Delta x} (u_{j+1}^n - u_{j-1}^n)$$

- (b)

$$u_j^{n+1} = \frac{1}{2} u_{j+1}^n + \frac{1}{2} u_{j-1}^n - \frac{\Delta t}{2\Delta x} (u_{j+1}^n - u_{j-1}^n)$$